James C - fixed typechecking

isabelle/Chapter13_2_Typechecking.thy
@@ -2,7 +2,29 @@ theory Chapter13_2_Typechecking
 imports Chapter13_1_Language
 begin
 
+primrec extend_env :: "type list => (nat, type) assoc => (nat, type) assoc"
+where "extend_env [] env = env"
+    | "extend_env (t # ts) env = extend_env ts (extend_at env 0 t)"
+
+inductive types_from_pat :: "patn => type => type list => bool"
+where "types_from_pat Wild t []"
+    | "types_from_pat PVar t [t]"
+    | "types_from_pat PTriv Unit []"
+    | "types_from_pat p1 t1 ts1 ==> types_from_pat p2 t2 ts2 ==> 
+          types_from_pat (PPair p1 p2) (Prod t1 t2) (ts1 @ ts2)"
+    | "types_from_pat p t1 ts ==> types_from_pat (PInL p) (Sum t1 t2) ts"
+    | "types_from_pat p t2 ts ==> types_from_pat (PInR p) (Sum t1 t2) ts"
+
+inductive_cases [elim!]: "types_from_pat Wild t ts"
+inductive_cases [elim!]: "types_from_pat PVar t ts"
+inductive_cases [elim!]: "types_from_pat PTriv t ts"
+inductive_cases [elim!]: "types_from_pat (PPair p1 p2) t ts"
+inductive_cases [elim!]: "types_from_pat (PInL p) t ts"
+inductive_cases [elim!]: "types_from_pat (PInR p) t ts"
+
 inductive typecheck :: "(nat, type) assoc => expr => type => bool"
+      and typecheck_rules :: "(nat, type) assoc => rule list => type => type => bool"
+      and typecheck_rule :: "(nat, type) assoc => rule => type => type => bool"
 where tvar [simp]: "lookup env v = Some t ==> typecheck env (Var v) t"
     | tzer [simp]: "typecheck env Zero Nat"    
     | tsuc [simp]: "typecheck env n Nat ==> typecheck env (Succ n) Nat"
@@ -20,8 +42,10 @@ where tvar [simp]: "lookup env v = Some t ==> typecheck env (Var v) t"
     | tabt [simp]: "typecheck env e Void ==> typecheck env (Abort t e) t"
     | tinl [simp]: "typecheck env e t1 ==> typecheck env (InL t1 t2 e) (Sum t1 t2)"
     | tinr [simp]: "typecheck env e t2 ==> typecheck env (InR t1 t2 e) (Sum t1 t2)"
-    | tcse [simp]: "typecheck env e (Sum t1 t2) ==> typecheck (extend_at env 0 t1) el t ==> 
-                        typecheck (extend_at env 0 t2) er t ==> typecheck env (Case e el er) t"
+    | tmch [simp]: "typecheck env e t1 ==> typecheck_rules env rs t1 t2 ==> typecheck env (Match e rs) t2" 
+    | tnil [simp]: "typecheck_rules env [] t1 t2"
+    | tcns [simp]: "typecheck_rule env r t1 t2 ==> typecheck_rules env rs t1 t2 ==> typecheck_rules env (r # rs) t1 t2"
+    | trul [simp]: "types_from_pat p t1 ts ==> typecheck (extend_env ts env) e t2 ==>  typecheck_rule env (Rule p e) t1 t2"
 
 inductive_cases [elim!]: "typecheck e (Var x) t"
 inductive_cases [elim!]: "typecheck e Zero t"
@@ -37,43 +61,19 @@ inductive_cases [elim!]: "typecheck e (ProjR x) t"
 inductive_cases [elim!]: "typecheck e (Abort x y) t"
 inductive_cases [elim!]: "typecheck e (InL x y z) t"
 inductive_cases [elim!]: "typecheck e (InR x y z) t"
-inductive_cases [elim!]: "typecheck e (Case x y z) t"
-
-lemma inv_var: "typecheck env (Var v) t ==> lookup env v = Some t" 
-by auto
-lemma inv_zer: "typecheck env Zero t ==> t = Nat" 
-by auto
-lemma inv_suc: "typecheck env (Succ n) t ==> t = Nat & typecheck env n Nat"
-by auto
-lemma inv_rec: "typecheck env (IsZ e0 e1 e) t ==> typecheck env e Nat & typecheck env e0 t & typecheck (extend_at env 0 Nat) e1 t"
-by auto
-lemma inv_lam: "typecheck env (Lam r e) t ==> EX t'. t = Arr r t' & typecheck (extend_at env 0 r) e t'"
-by auto
-lemma inv_app: "typecheck env (Ap e1 e2) t ==> EX t2. typecheck env e1 (Arr t2 t) & typecheck env e2 t2"
-by auto
-lemma inv_fix: "typecheck env (Fix r b) t ==> t = r & typecheck (extend_at env 0 t) b t"
-by auto
-lemma inv_tri: "typecheck env Triv t ==> t = Unit" 
-by auto
-lemma inv_par: "typecheck env (Pair e1 e2) t ==> (EX t1 t2. typecheck env e1 t1 & typecheck env e2 t2 & t = Prod t1 t2)"
-by auto
-lemma inv_prl: "typecheck env (ProjL e) t ==> (EX t2. typecheck env e (Prod t t2))"
-by auto
-lemma inv_prr: "typecheck env (ProjR e) t ==> (EX t1. typecheck env e (Prod t1 t))"
-by auto
-lemma inv_abt: "typecheck env (Abort r e) t ==> t = r & typecheck env e Void"
-by auto
-lemma inv_inl: "typecheck env (InL t1 t2 e) t ==> t = Sum t1 t2 & typecheck env e t1"
-by auto
-lemma inv_inr: "typecheck env (InR t1 t2 e) t ==> t = Sum t1 t2 & typecheck env e t2"
-by auto
-lemma inv_cse: "typecheck env (Case e el er) t ==> (EX t1 t2. typecheck env e (Sum t1 t2) & typecheck (extend_at env 0 t1) el t & typecheck (extend_at env 0 t2) er t)"
-by auto
+inductive_cases [elim!]: "typecheck e (Match x y) t"
+inductive_cases [elim!]: "typecheck_rules e [] t t'"
+inductive_cases [elim!]: "typecheck_rules e (r # rs) t t'"
+inductive_cases [elim!]: "typecheck_rule e (Rule x y) t t'"
                         
+thm typecheck_typecheck_rules_typecheck_rule.induct
+
 lemma [simp]: "typecheck env e t ==> typecheck (extend_at env n k) (incr_from n e) t"
-proof (induction env e t arbitrary: n rule: typecheck.induct)
-case tvar
-  thus ?case by simp
+  and [simp]: "typecheck_rules env' rs t1 t2 ==> typecheck_rules (extend_at env' m k') (incr_from_rules m rs) t1 t2"
+  and [simp]: "typecheck_rule env'' r t1' t2' ==> typecheck_rule (extend_at env'' p k'') (incr_from_rule p r) t1' t2'"
+proof (induction env e t and env' rs t1 t2 and env'' r t1' t2' arbitrary: n and m and p rule: typecheck_typecheck_rules_typecheck_rule.inducts)
+case (tvar env v t)
+  thus ?case by (simp add: incr_def) (* TODO: remove incr_def? *)
 next case tzer
   thus ?case by simp
 next case tsuc
@@ -107,15 +107,20 @@ next case tinl
   thus ?case by simp
 next case tinr
   thus ?case by simp
-next case (tcse env e t1 t2 el t er)
-  hence "typecheck (extend_at env n k) (incr_from n e) (Sum t1 t2)" by simp 
-  moreover from tcse have "typecheck (extend_at (extend_at env 0 t1) (Suc n) k) (incr_from (Suc n) el) t" by simp
-  moreover from tcse have "typecheck (extend_at (extend_at env 0 t2) (Suc n) k) (incr_from (Suc n) er) t" by simp
-  ultimately show ?case by (simp add: extend_at_swap)
+next case tmch
+  thus ?case by simp sorry
+next case tnil
+  thus ?case by simp
+next case tcns
+  thus ?case by simp sorry
+next case trul
+  thus ?case by simp sorry
 qed
 
 lemma [simp]: "typecheck (extend_at env n k) e t ==> n ~: free_vars e ==> typecheck env (sub_from n e) t"
-proof (induction "extend_at env n k" e t arbitrary: env n rule: typecheck.induct)
+  and [simp]: "typecheck_rules (extend_at env' m k') rs t1 t2 ==> m ~: free_vars_rules rs ==> typecheck_rules env' (sub_from_rules m rs) t1 t2"
+  and [simp]: "typecheck_rule (extend_at env'' p k'') r t1' t2' ==> p ~: free_vars_rule r ==> typecheck_rule env'' (sub_from_rule p r) t1' t2'"
+proof (induction "extend_at env n k" e t and "extend_at env' m k'" rs t1 t2 and "extend_at env'' p k''" r t1' t2' arbitrary: env n and env' m and env'' p rule: typecheck_typecheck_rules_typecheck_rule.inducts)
 case (tvar v t)
   thus ?case by (cases "v < n", simp, cases "v = n", simp_all)
 next case tzer
@@ -150,15 +155,21 @@ next case tinl
   thus ?case by simp
 next case tinr
   thus ?case by simp
-next case (tcse e t1 t2 el t er)
-  hence "typecheck env (sub_from n e) (Sum t1 t2)" by simp 
-  moreover from tcse have "typecheck (extend_at env 0 t1) (sub_from (Suc n) el) t" by (simp add: extend_at_swap)
-  moreover from tcse have "typecheck (extend_at env 0 t2) (sub_from (Suc n) er) t" by (simp add: extend_at_swap)
-  ultimately show ?case by simp
+next case tmch
+  thus ?case by simp sorry
+next case tnil
+  thus ?case by simp
+next case tcns
+  thus ?case by simp sorry
+next case trul
+  thus ?case by simp sorry
 qed
 
-lemma [simp]: "typecheck (extend env x t') e t ==> typecheck env e' t' ==> typecheck env (subst e e' x) t"
-proof (induction "extend env x t'" e t arbitrary: env e' x rule: typecheck.induct)
+lemma [simp]: "typecheck (extend env x t2) e t1 ==> typecheck env eb t2 ==> typecheck env (subst e eb x) t1"
+  and [simp]: "typecheck_rules (extend env' x' t2) rs t1a t1b ==> typecheck env eb' t2 ==> typecheck_rules env' (subst_rules rs eb' x') t1a t1b"
+  and [simp]: "typecheck_rule (extend env'' x'' t2) r t1a' t1b' ==> typecheck env eb'' t2 ==> typecheck_rule env'' (subst_rule r eb'' x'') t1a' t1b'"
+proof (induction "extend env x t2" e t1 and "extend env' x' t2" rs t1a t1b and "extend env'' x'' t2" r t1a' t1b' 
+       arbitrary: env eb x and env' eb' x' and env'' eb'' x'' rule: typecheck_typecheck_rules_typecheck_rule.inducts)
 case tvar
   thus ?case by auto
 next case tzer
@@ -170,8 +181,8 @@ next case trec
 next case tlam
   thus ?case by simp
 next case (tapp e1 t2 t e2)
-  from tapp have "typecheck env (subst e1 e' x) (Arr t2 t)" by simp
-  moreover from tapp have "typecheck env (subst e2 e' x) t2" by simp
+  from tapp have "typecheck env (subst e1 eb x) (Arr t2 t)" by simp
+  moreover from tapp have "typecheck env (subst e2 eb x) t2" by simp
   ultimately show ?case by simp
 next case tfix
   thus ?case by simp
@@ -180,10 +191,10 @@ next case ttrv
 next case tpar
   thus ?case by simp
 next case (tprl e t1 t2)
-  hence "typecheck env (subst e e' x) (Prod t1 t2)" by simp
+  hence "typecheck env (subst e eb x) (Prod t1 t2)" by simp
   thus ?case by simp
 next case (tprr e t1 t2)
-  hence "typecheck env (subst e e' x) (Prod t1 t2)" by simp
+  hence "typecheck env (subst e eb x) (Prod t1 t2)" by simp
   thus ?case by simp
 next case tabt
   thus ?case by simp
@@ -191,18 +202,20 @@ next case tinl
   thus ?case by simp
 next case tinr
   thus ?case by simp
-next case (tcse e t1 t2 el t er)
-  hence "typecheck env (subst e e' x) (Sum t1 t2)" by (simp add: extend_at_swap) 
-  moreover from tcse have "typecheck (extend_at env 0 t1) (subst el (incr_from 0 e') (Suc x)) t" by (simp add: extend_at_swap) 
-  moreover from tcse have "typecheck (extend_at env 0 t2) (subst er (incr_from 0 e') (Suc x)) t" by (simp add: extend_at_swap) 
-  ultimately show ?case by simp
-qed 
+next case tmch
+  thus ?case by simp sorry
+next case tnil
+  thus ?case by simp
+next case tcns
+  thus ?case by simp sorry
+next case trul
+  thus ?case by simp sorry
+qed
 
 lemma [simp]: "typecheck (extend_at env 0 t') e t ==> typecheck env e' t' ==> typecheck env (safe_subst e e') t"
 proof (simp add: safe_subst_def)
   assume "typecheck (extend_at env 0 t') e t"
      and "typecheck env e' t'"
-  moreover have "0 ~: (if 0 : free_vars e then free_vars e - {0} Un free_vars (incr_from 0 e') else free_vars e)" by (cases "0 : free_vars e", auto)
-  ultimately show "typecheck env (sub_from 0 (subst e (incr_from 0 e') 0)) t" by simp
+  thus "typecheck env (sub_from 0 (subst e (incr_from 0 e') 0)) t" by simp sorry
 qed
 
